Dafny/examples/BasicBugSet/simpleBugBenignLemmas.i.dfy
@@ -18,21 +18,22 @@ module simpleBugBenignLemmas{
         requires s.o.Nil?;
 
         ensures  forall input :: (validInput(s,input) && OperandContents(s,input).val < 2 && ValidBehaviorNonTrivial(b) &&BehaviorEvalsCode(codeVuln(input),b)) 
-                                  ==> (behaviorOutput(b) == [Nil,Nil,Nil,Out((Int(1,IntType(1,false)))),Out((Int(1,IntType(1,false))))]);
+                                  ==> (behaviorOutput(b) == validOutput());
         ensures  forall input :: (validInput(s,input) && OperandContents(s,input).val >= 2 && ValidBehaviorNonTrivial(b) && BehaviorEvalsCode(codeVuln(input),b)) 
-                                  ==> (behaviorOutput(b) == [Nil,Nil,Nil,Out((Int(0,IntType(1,false)))),Out((Int(0,IntType(1,false))))]);
+                                  ==> (behaviorOutput(b) == invalidOutput());
     {
         var inputWitness := D(Int(1,IntType(4,false)));
         assert validInput(s,inputWitness);
+
         forall input | validInput(s,input) && OperandContents(s,input).val < 2 && ValidBehaviorNonTrivial(b) && BehaviorEvalsCode(codeVuln(input),b)
-            ensures (behaviorOutput(b) == [Nil,Nil,Nil,Out((Int(1,IntType(1,false)))),Out((Int(1,IntType(1,false))))]);
+            ensures (behaviorOutput(b) == validOutput());
         {
             var input :| validInput(s,input) && OperandContents(s,input).val < 2 && BehaviorEvalsCode(codeVuln(input),b);
             var b' := unwrapVulnBehaviors(s,input);
             behaviorThatEvalsSameCodeWithSameInitIsEqual(s,codeVuln(input),b');
         }
         forall input | validInput(s,input) && OperandContents(s,input).val >= 2 && ValidBehaviorNonTrivial(b) && BehaviorEvalsCode(codeVuln(input),b)
-            ensures (behaviorOutput(b) == [Nil,Nil,Nil,Out((Int(0,IntType(1,false)))),Out((Int(0,IntType(1,false))))]);
+            ensures (behaviorOutput(b) == invalidOutput());
         {
             var input :| validInput(s,input) && OperandContents(s,input).val >= 2 && BehaviorEvalsCode(codeVuln(input),b);
             var b' := unwrapVulnBehaviors(s,input);
@@ -42,48 +43,45 @@ module simpleBugBenignLemmas{
     }
 lemma existsVulnBehavor(s:state,b:behavior,vulnBehaviors:set<behavior>,input:operand)
         requires ValidState(s);
-        requires validPatchBehavior(b)
+        requires validVulnBehavior(b)
         requires |b| > 0;
         requires |vulnBehaviors| > 0; 
         requires b[0] == s;
-        requires BehaviorEvalsCode(codePatch(input),b) && |b| > 0 && validInput(b[0],input);
-        requires forall v :: v in vulnBehaviors <==> (exists input :: validInput(s,input) && ValidBehaviorNonTrivial(v) && BehaviorEvalsCode(codeVuln(input),v) && v[0] == s)
-        requires forall input :: validInput(s,input) ==> (exists b :: ValidBehaviorNonTrivial(b) && BehaviorEvalsCode(codeVuln(input),b) && b[0] == s)
+        requires BehaviorEvalsCode(codeVuln(input),b) && |b| > 0 && validInput(b[0],input);
+        requires nonTrivialBehaviorPreconditionsVuln(s,vulnBehaviors);
         ensures exists vuln, vulnIn :: vuln in vulnBehaviors && validInput(s,vulnIn)  && OperandContents(s,vulnIn).val < 2 && BehaviorEvalsCode(codeVuln(vulnIn),vuln);
 
     {
         reveal_BehaviorEvalsCode();
-        // validInputVulnImpliesBehavior(s);
-        // var input :| BehaviorEvalsCode(codePatch(input),b) && |b| > 0 && validInput(b[0],input);
-        var b' := unwrapPatchBehaviors(s,input);
+        reveal_nonTrivialBehaviorPreconditionsVuln();
+        validInputVulnImpliesBehavior(s);
+        var b' := unwrapVulnBehaviors(s,input);
         assert exists vuln, vulnIn :: vuln in vulnBehaviors && validInput(s,vulnIn)  && OperandContents(s,vulnIn).val < 2 && BehaviorEvalsCode(codeVuln(vulnIn),vuln);
     }
 
     lemma vulnBehaviorIncludesPatchedBehavior(s:state,b:behavior,vulnBehaviors:set<behavior>)
         requires ValidState(s);
         requires validPatchBehavior(b)
-        requires |b| > 0;
         requires |vulnBehaviors| > 0; 
-        requires b[0] == s;
-        requires forall v :: v in vulnBehaviors <==> (exists input :: validInput(s,input) && ValidBehaviorNonTrivial(v) && BehaviorEvalsCode(codeVuln(input),v) && v[0] == s)
-        ensures exists v :: (v in vulnBehaviors && equalOutput(behaviorOutput(v), [Nil,Nil,Nil,Out((Int(1,IntType(1,false)))),Out((Int(1,IntType(1,false))))]));
+        requires nonTrivialBehaviorPreconditionsVuln(s,vulnBehaviors);
+        ensures exists v :: (v in vulnBehaviors && equalOutput(behaviorOutput(v), validOutput()));
 
     {
+        reveal_nonTrivialBehaviorPreconditionsVuln();
         reveal_BehaviorEvalsCode();
         validInputVulnImpliesBehavior(s);
-        var input :| BehaviorEvalsCode(codePatch(input),b) && |b| > 0 && validInput(b[0],input);
-        var b' := unwrapPatchBehaviors(s,input);
+        assert nonTrivialBehaviorPreconditionsVuln(s,vulnBehaviors);
+        var vulnB :| vulnB in vulnBehaviors;
+        var input :| validInput(s,input) &&  ValidBehaviorNonTrivial(vulnB) && BehaviorEvalsCode(codeVuln(input),vulnB) && vulnB[0] == s;
+        var b' := unwrapVulnBehaviors(s,input);
        
-        existsVulnBehavor(s,b,vulnBehaviors,input);
+        existsVulnBehavor(s,vulnB,vulnBehaviors,input);
         var vuln, vulnIn :| vuln in vulnBehaviors && validInput(s,vulnIn)  && OperandContents(s,vulnIn).val < 2 && BehaviorEvalsCode(codeVuln(vulnIn),vuln);
         possibleVulnOutputs(s,vuln);
-        assert equalOutput(behaviorOutput(vuln),[Nil,Nil,Nil,Out((Int(1,IntType(1,false)))),Out((Int(1,IntType(1,false))))]);
+        assert equalOutput(behaviorOutput(vuln),validOutput());
         
-        assert vuln in vulnBehaviors && equalOutput(behaviorOutput(vuln), behaviorOutput(b));
-        assert exists v :: (v in vulnBehaviors && equalOutput(behaviorOutput(v), behaviorOutput(b)));
         var vulnOut := allBehaviorOutputSet(vulnBehaviors);
-        assert forall v :: v in vulnBehaviors ==> behaviorOutput(v) in vulnOut;
-        assert [Nil,Nil,Nil,Out((Int(1,IntType(1,false)))),Out((Int(1,IntType(1,false))))] in vulnOut;
+        assert validOutput() in vulnOut;
 
     }
 
@@ -92,17 +90,16 @@ lemma existsVulnBehavor(s:state,b:behavior,vulnBehaviors:set<behavior>,input:ope
         requires |patchBehaviors| == 0
         requires |patchOut| == 0
         requires ValidState(s);
-        requires forall b :: b in vulnBehaviors <==> (exists input :: validInput(s,input) &&  ValidBehaviorNonTrivial(b) && BehaviorEvalsCode(codeVuln(input),b) && b[0] == s)
-        requires forall b :: b in patchBehaviors <==> (exists input :: validInput(s,input) &&  ValidBehaviorNonTrivial(b) && BehaviorEvalsCode(codePatch(input),b) && b[0] == s)
-
-        ensures forall p :: p in patchOut ==> p in vulnOut
+        requires nonTrivialBehaviorPreconditions(s,vulnBehaviors,patchBehaviors);
+        ensures forall postOutput :: postOutput in patchOut ==> postOutput in vulnOut
         {
-           
+            reveal_nonTrivialBehaviorPreconditionsVuln();
+            reveal_nonTrivialBehaviorPreconditionsPatch();
             assert |patchBehaviors| == 0;
             assert |patchOut| == 0;
-            assert forall p :: p in patchBehaviors ==> p in vulnBehaviors;
-            assert forall p :: p in patchBehaviors ==> (exists v :: v in vulnBehaviors && equalOutput(behaviorOutput(v), behaviorOutput(p)));
-            assert forall p :: p in patchOut ==> p in vulnOut;
+            assert forall postB :: postB in patchBehaviors ==> postB in vulnBehaviors;
+            assert forall postB :: postB in patchBehaviors ==> (exists preB :: preB in vulnBehaviors && equalOutput(behaviorOutput(preB), behaviorOutput(postB)));
+            assert forall postOutput :: postOutput in patchOut ==> postOutput in vulnOut;
             
         }
 
@@ -112,62 +109,40 @@ lemma existsVulnBehavor(s:state,b:behavior,vulnBehaviors:set<behavior>,input:ope
         requires |patchBehaviors| > 0;
         requires vulnOut == allBehaviorOutputSet(vulnBehaviors);
         requires patchOut ==  allBehaviorOutputSet(patchBehaviors);
-        // requires expandedAllBehaviorsSurjective(vulnBehaviors,vulnOut);
-        // requires expandedAllBehaviorsSurjective(patchBehaviors,patchOut);
 
-        // requires SurjectiveOver(vulnBehaviors,vulnOut, x => behaviorOutput(x));
-        // requires SurjectiveOver(patchBehaviors,patchOut, x => behaviorOutput(x));
-        ensures forall p :: p in patchBehaviors ==> exists v :: (v in vulnBehaviors && equalOutput(behaviorOutput(v), behaviorOutput(p)));
-        ensures forall p :: p in patchBehaviors ==> equalOutput(behaviorOutput(p),[Nil,Nil,Nil,Out((Int(1,IntType(1,false)))),Out((Int(1,IntType(1,false))))]);
-        ensures forall p :: p in patchBehaviors ==> behaviorOutput(p) in vulnOut;
-        ensures forall p :: p in patchBehaviors ==> behaviorOutput(p) in patchOut;
+        ensures forall postB :: postB in patchBehaviors ==> exists preB :: (preB in vulnBehaviors && equalOutput(behaviorOutput(preB), behaviorOutput(postB)));
+        ensures forall postB :: postB in patchBehaviors ==> equalOutput(behaviorOutput(postB),validOutput());
+        ensures forall postB :: postB in patchBehaviors ==> behaviorOutput(postB) in vulnOut;
+        ensures forall postB :: postB in patchBehaviors ==> behaviorOutput(postB) in patchOut;
     {
         reveal_BehaviorEvalsCode();
-        // validInputVulnImpliesBehavior(s);
-        // reveal_expandedAllBehaviorsSurjective();
         reveal_nonTrivialBehaviorPreconditionsVuln();
         reveal_nonTrivialBehaviorPreconditionsPatch();
-        // reveal_allBehaviorOutputSet();
         assert |patchBehaviors| > 0;
-        assert forall p :: p in patchBehaviors ==> validPatchBehavior(p);
+        assert forall postB :: postB in patchBehaviors ==> validPatchBehavior(postB);
 
-        // allBehaviorEqualityIsInjective(vulnBehaviors,vulnOut);
-        //         assert SurjectiveOver(vulnBehaviors,vulnOut, x => behaviorOutput(x));// ==> forall y :: y in vulnOut ==> (exists x :: x in vulnBehaviors && behaviorOutput(x) == y);
-
-        // allBehaviorsSetSurjective(vulnBehaviors,vulnOut);
-        // assert  
-        // assert forall x :: x in allBehaviors(patchBehaviors) ==> equalOutput(x,[Nil,Nil,Nil,Out((Int(1,IntType(1,false)))),Out((Int(1,IntType(1,false))))]);
-        forall p | p in patchBehaviors
-            ensures exists v :: (v in vulnBehaviors && equalOutput(behaviorOutput(v), behaviorOutput(p)));
-            ensures equalOutput(behaviorOutput(p),[Nil,Nil,Nil,Out((Int(1,IntType(1,false)))),Out((Int(1,IntType(1,false))))]);
-            ensures behaviorOutput(p) in vulnOut;
-            ensures behaviorOutput(p) in patchOut;
+        forall postB | postB in patchBehaviors
+            ensures exists preB :: (preB in vulnBehaviors && equalOutput(behaviorOutput(preB), behaviorOutput(postB)));
+            ensures equalOutput(behaviorOutput(postB),validOutput());
+            ensures behaviorOutput(postB) in vulnOut;
+            ensures behaviorOutput(postB) in patchOut;
             {
 
-                var input :| BehaviorEvalsCode(codePatch(input),p) && |p| > 0 && validInput(p[0],input);
+                var input :| BehaviorEvalsCode(codePatch(input),postB) && |postB| > 0 && validInput(postB[0],input);
                 var b' := unwrapPatchBehaviors(s,input);
-                assert equalOutput(behaviorOutput(p),[Nil,Nil,Nil,Out((Int(1,IntType(1,false)))),Out((Int(1,IntType(1,false))))]);
+                assert equalOutput(behaviorOutput(postB),validOutput());
 
-                vulnBehaviorIncludesPatchedBehavior(s,p,vulnBehaviors);
-                assert exists v :: (v in vulnBehaviors && equalOutput(behaviorOutput(v), [Nil,Nil,Nil,Out((Int(1,IntType(1,false)))),Out((Int(1,IntType(1,false))))]));
-                var v :| (v in vulnBehaviors && equalOutput(behaviorOutput(v), [Nil,Nil,Nil,Out((Int(1,IntType(1,false)))),Out((Int(1,IntType(1,false))))]));
-                assert behaviorOutput(v) in vulnOut;
+                vulnBehaviorIncludesPatchedBehavior(s,postB,vulnBehaviors);
+                assert exists preB :: (preB in vulnBehaviors && equalOutput(behaviorOutput(preB), validOutput()));
+                var preB :| (preB in vulnBehaviors && equalOutput(behaviorOutput(preB), validOutput()));
+                assert behaviorOutput(preB) in vulnOut;
                 
-                transitiveEquality(behaviorOutput(p),behaviorOutput(v),[Nil,Nil,Nil,Out((Int(1,IntType(1,false)))),Out((Int(1,IntType(1,false))))]);
-                assert behaviorOutput(p) == behaviorOutput(v);
-                equalOutputIsTransitiveSet(behaviorOutput(v),behaviorOutput(p),vulnOut);
-                assert behaviorOutput(p) in vulnOut;
+                transitiveEquality(behaviorOutput(postB),behaviorOutput(preB),validOutput());
+                assert behaviorOutput(postB) == behaviorOutput(preB);
+                equalOutputIsTransitiveSet(behaviorOutput(preB),behaviorOutput(postB),vulnOut);
+                assert behaviorOutput(postB) in vulnOut;
             }
-        assert forall p :: p in patchBehaviors ==> behaviorOutput(p) in vulnOut;
-        // assert forall p :: behaviorOutput(p) in patchOut ==> behaviorOutput(p) in vulnOut;
-        // forall p | p in patchOut
-        // {
-        //     assert exists x :: x in patchBehaviors && behaviorOutput(x) == p;
-
-        //     assert equalOutput(p, [Nil,Nil,Nil,Out((Int(1,IntType(1,false)))),Out((Int(1,IntType(1,false))))]);
-        // }
-        // assert forall p :: p in patchOut ==> equalOutput(p, [Nil,Nil,Nil,Out((Int(1,IntType(1,false)))),Out((Int(1,IntType(1,false))))]);
-               
+        assert forall postB :: postB in patchBehaviors ==> behaviorOutput(postB) in vulnOut;
             
     }
 
