Dafny/examples/BasicBugSet/simpleBugProperties.i.dfy
@@ -1,27 +1,22 @@
 include "simpleBugBenignLemmas.i.dfy"
-include "simpleBugCompleteLemmasV2.i.dfy"
+include "simpleBugCompleteLemmas.i.dfy"
+include "simpleBugGeneral.i.dfy"
 include "simpleBugCode.i.dfy"
 include "../../LLVM/llvmREFACTOR.i.dfy"
 include "../../LLVM/types.dfy"
-include "simpleBugGeneral.i.dfy"
 include "../../Libraries/Seqs.s.dfy"
 include "../../Libraries/Sets.i.dfy"
 
 
 module simpleBugProperties{
     import opened simpleBugBenignLemmas
-    import opened simpleBugCompleteLemmasV2
+    import opened simpleBugCompleteLemmas
     import opened simpleBugCode
+    import opened simpleBugGeneral
     import opened LLVM_defRE
     import opened types
-    import opened simpleBugGeneral
     import opened Collections__Seqs_s
     import opened Collections__Sets_i
-
-
-
-
-
 
 ///////////////////////////////
 
@@ -37,11 +32,11 @@ module simpleBugProperties{
         var patchOut :=  allBehaviorOutputSet(patchBehaviors);
         if (|patchBehaviors| == 0){
             patchIsBenignTrivial(s,vulnBehaviors,patchBehaviors,vulnOut,patchOut);
-            assert forall p :: p in patchOut ==> p in vulnOut;
+            assert forall postOutput :: postOutput in patchOut ==> postOutput in vulnOut;
         }else{
             assert |patchBehaviors| > 0;
             patchIsBenignNonTrivial(s,vulnBehaviors,patchBehaviors,vulnOut,patchOut);
-            assert forall p :: p in patchOut ==> p in vulnOut;
+            assert forall postOutput :: postOutput in patchOut ==> postOutput in vulnOut;
         }
     }
 
@@ -61,21 +56,21 @@ module simpleBugProperties{
         
         var result := LV("result");
          if (|patchBehaviors| == 0){
-             assert forall p :: MiniSpec(p) ==> !(p in patchBehaviors);
+             assert forall behavior :: MiniSpec(behavior) ==> !(behavior in patchBehaviors);
          } else {
              assert |patchBehaviors| > 0;
-             assert forall q :: MiniSpec(q) ==> RemovedBehaviors(q);
-             forall p | p in patchBehaviors
-                ensures !MiniSpec(p);
+             assert forall behavior :: MiniSpec(behavior) ==> RemovedBehaviors(behavior);
+             forall postB | postB in patchBehaviors
+                ensures !MiniSpec(postB);
                 {  
-                    var input :| BehaviorEvalsCode(codePatch(input),p) && |p| > 0 && validInput(p[0],input);
-                    var b' := unwrapPatchBehaviors(s,input);
-                    behaviorThatEvalsSameCodeWithSameInitIsEqual(s,codePatch(input),b');
-                    assert !RemovedBehaviors(p);
-                    assert !MiniSpec(p);
+                    var input :| BehaviorEvalsCode(codePatch(input),postB) && |postB| > 0 && validInput(postB[0],input);
+                    var postBWitness := unwrapPatchBehaviors(s,input);
+                    behaviorThatEvalsSameCodeWithSameInitIsEqual(s,codePatch(input),postBWitness);
+                    assert !RemovedBehaviors(postB);
+                    assert !MiniSpec(postB);
                 }
                 
-                assert forall p :: MiniSpec(p) ==> !(p in patchBehaviors);
+                assert forall behavior :: MiniSpec(behavior) ==> !(behavior in patchBehaviors);
              }
          }
 
@@ -124,111 +119,46 @@ module simpleBugProperties{
 
         requires nonTrivialBehaviorPreconditions(s,vulnBehaviors,patchBehaviors)
         requires |patchBehaviors|  > 0
-        // requires completePatch(vulnBehaviors,patchBehaviors);
         //
-        // requires nonTrivialBehaviorPreconditions(s,vulnBehaviors,patchBehaviors)
-
-        // ensures safePatch(a,b);
+        ensures |MakeSubset(vulnBehaviors, x => !MiniSpec(x))|> 0 ==> safePatchMS(vulnBehaviors,patchBehaviors); 
     {
         var aModuloMS := findModMsSet(s,vulnBehaviors);
-        // var aModuloMS := MakeSubset(vulnBehaviors, x => !MiniSpec(x));
         var aOutMS := allBehaviorOutputSet(aModuloMS);
         var aOut := allBehaviorOutputSet(vulnBehaviors);
         var bOut := allBehaviorOutputSet(patchBehaviors);
 
         assert forall p :: behaviorOutput(p) in aOutMS ==> behaviorOutput(p) in bOut;
-        // assert (forall p :: behaviorOutput(p) in bOut ==> behaviorOutput(p) in aOutMS) ==> safePatchMS(vulnBehaviors,patchBehaviors);
 
         assert forall p :: behaviorOutput(p) in bOut ==> behaviorOutput(p) in aOut;
         assert  forall p :: MiniSpec(p) ==> !(p in patchBehaviors);
-        subsetOfBehaviorImpliesSubsetOfOutputFull(vulnBehaviors,aModuloMS,aOut,aOutMS,x => !MiniSpec(x));
-        assert forall p :: p in aOutMS ==> p in aOut;
+        // subsetOfBehaviorImpliesSubsetOfOutputFull(vulnBehaviors,aModuloMS,aOut,aOutMS,x => !MiniSpec(x));
+        // assert forall p :: p in aOutMS ==> p in aOut;
 
-        // assert (forall p :: behaviorOutput(p) in bOut ==> behaviorOutput(p) in aOut) ;
-        // assert aOutMS == allBehaviorOutputSet(aModuloMS);
-        // assert bOut ==  allBehaviorOutputSet(patchBehaviors);
-        // assert ValidState(s);
-        // assert forall p :: p in aModuloMS ==> !MiniSpec(p);
-        // assert forall b :: b in aModuloMS ==> (exists input :: validInput(s,input) &&  ValidBehaviorNonTrivial(b) && BehaviorEvalsCode(codeVuln(input),b) && b[0] == s);
-        // assert nonTrivialBehaviorPreconditionsPatch(s,patchBehaviors);
-        // assert |patchBehaviors|  > 0;
         if(|aModuloMS| > 0)
         {
             patchBehaviorsInVulnModMSBehaviors(s,aModuloMS,patchBehaviors,aOutMS,bOut);
             assert forall p :: p in bOut  ==> p in aOutMS; 
             assert safePatchMS(vulnBehaviors,patchBehaviors);
         }
-        // patchIsSafeHelper(s,aModuloMS,patchBehaviors,aOutMS,bOut);
-        // assert |aModuloMS| > 0 ==>
-        // assert (|aModuloMS| > 0) ==> (forall p :: p in bOut  ==> p in aOutMS); 
-        // assert (|aModuloMS| > 0) ==>  safePatchMS(vulnBehaviors,patchBehaviors);
-
-        // assert false;
-        // assert |patchBehaviors|  > 0;
-        // assert forall p :: behaviorOutput(p) in bOut ==> MiniSpec(p);
-
-
-        // assert safePatchMS(vulnBehaviors,patchBehaviors);
 
     }
 
-
-    // lemma patchIsSafeHelper(s:state,aModuloMS:set<behavior>,patchBehaviors:set<behavior>,vulnModMsOut:set<seq<output>>,patchOut:set<seq<output>>)
-    //     requires vulnModMsOut == allBehaviorOutputSet(aModuloMS);
-    //     requires patchOut ==  allBehaviorOutputSet(patchBehaviors);
-    //     requires ValidState(s);
-    //     requires forall p :: p in aModuloMS ==> !MiniSpec(p);
-    //     requires forall b :: b in aModuloMS ==> (exists input :: validInput(s,input) &&  ValidBehaviorNonTrivial(b) && BehaviorEvalsCode(codeVuln(input),b) && b[0] == s)
-    //     requires nonTrivialBehaviorPreconditionsPatch(s,patchBehaviors);
-    //     requires |patchBehaviors|  > 0
-    //     ensures (|aModuloMS| > 0) ==> (forall p :: p in patchOut  ==> p in vulnModMsOut);
-    //     // ensures benignPatch(vulnBehaviors,patchBehaviors)
-    // {
-    //     reveal_nonTrivialBehaviorPreconditionsVuln();
-    //     reveal_nonTrivialBehaviorPreconditionsPatch();
-    //     // reveal_BehaviorEvalsCode();
-    //     // reveal_ValidBehavior();
-    //     reveal_behaviorOutput();
-    //     // var vulnModMs := findModMsSet(s,vulnBehaviors);
-    //     // var vulnModMsOut := allBehaviorOutputSet(aModuloMS);
-    //     // var patchOut :=  allBehaviorOutputSet(patchBehaviors);
-
-    //     // assert vulnModMs ==  MakeSubset(vulnBehaviors, x => !MiniSpec(x));
-    //      if(|aModuloMS| == 0)
-    //      {
-    //         //   assert  forall p :: p in patchOut  ==> p in vulnModMsOut;
-    //      }
-    //     else{
-    //         assert |aModuloMS| > 0;
-    //         patchBehaviorsInVulnModMSBehaviors(s,aModuloMS,patchBehaviors,vulnModMsOut,patchOut);
-    //         assert  forall p :: p in patchOut  ==> p in vulnModMsOut;
-    //     }
-    // }
-
-    // forall p :: (behaviorOutput(p) in aOut && !MiniSpec(p)) ==> behaviorOutput(p) in bOut
-    // lemma patchIsComplete(s:state,vulnBehaviors:set<behavior>,patchBehaviors:set<behavior>)
-    //     requires ValidState(s);
-    //     requires nonTrivialBehaviorPreconditions(s,vulnBehaviors,patchBehaviors)
-    //     // ensures completePatch(vulnBehaviors,patchBehaviors)
-    // {
-    //     reveal_nonTrivialBehaviorPreconditionsVuln();
-    //     reveal_nonTrivialBehaviorPreconditionsPatch();
-    //     reveal_behaviorOutput();
-    //     // reveal_BehaviorEvalsCode();
-    //     var vulnOut := allBehaviorOutput(vulnBehaviors);
-    //     var patchOut :=  allBehaviorOutput(patchBehaviors);
-    //     // assert forall p :: behaviorOutput(p) in vulnOut <==> (exists i :: (i >= 0 && i < |vulnBehaviors|) && vulnOut[i] == behaviorOutput(vulnBehaviors[i]));
-    //     if(|vulnBehaviors| == 0){
-    //         patchIsCompleteTrivial(s,vulnBehaviors,patchBehaviors,vulnOut,patchOut);
-    //         assert (forall p :: (behaviorOutput(p) in vulnOut && !MiniSpec(p))  ==> behaviorOutput(p) in patchOut);
-
-    //     }
-    //      if (|patchBehaviors| > 0){
-    //         patchIsCompleteNonTrivial(s,vulnBehaviors,patchBehaviors,vulnOut,patchOut);
-    //         // assert (forall p :: (p in vulnBehaviors && !MiniSpec(p)) ==> p in patchBehaviors);
-    //         // assert (forall p :: (behaviorOutput(p) in vulnOut && !MiniSpec(p))  ==> behaviorOutput(p) in patchOut);
-    //      }
-    // }
-    
+    lemma fullPatchNonTrivial(vulnBehaviors:set<behavior>,patchBehaviors:set<behavior>)
+        requires |patchBehaviors|  > 0
+        requires |MakeSubset(vulnBehaviors, x => !MiniSpec(x))| > 0
+        ensures forall s :: nonTrivialBehaviorPreconditions(s,vulnBehaviors,patchBehaviors) ==> safePatchMS(vulnBehaviors,patchBehaviors); 
+    {
+        forall s | nonTrivialBehaviorPreconditions(s,vulnBehaviors,patchBehaviors)
+            ensures safePatchMS(vulnBehaviors,patchBehaviors); 
+            {
+                patchIsBenign(s,vulnBehaviors,patchBehaviors);
+                patchIsSuccessful(s,patchBehaviors);
+                patchIsComplete(s,vulnBehaviors,patchBehaviors);
+                assert benignPatch(vulnBehaviors,patchBehaviors);
+                assert successfulPatch(patchBehaviors);
+                assert completePatchMS(vulnBehaviors,patchBehaviors); 
+                fullPatch(s,vulnBehaviors,patchBehaviors);
+            }
+    }
 
 }
